with type annotations fixed, but disabled

ModularEngine/src/LogicEngine.FStar/interp.fst
@@ -4,13 +4,17 @@ open Types
 open Util
 open Marshall
 open State
+open Subst
 
-type substrate
 type vars = list var
 type substitutions = list substitution
 
-val me : principal 
-let me = Crypto.lookup_my_credentials ()
+type IsMe :: principal => E
+val me : p:principal{IsMe p}
+let me = 
+  let v = Crypto.lookup_my_credentials () in 
+    assume (IsMe v);
+    v
 
 type condition =
   | If   : polyterm -> condition
@@ -33,26 +37,28 @@ type communications = list communication
 (* -------------------------------------------------------------------------------- *)
 (* Spec: Validity of condition(s) *)
 (* -------------------------------------------------------------------------------- *)
+type Includes :: vars => vars => E (* TODO *)
+
 logic function CondSubst : condition -> substitution -> condition
-assume forall (i:infon). (CondSubst (If i) s) = (If (PolySubst i s))
-assume forall (i:infon). (CondSubst (Upon i) s) = (Upon (PolySubst i s))
+assume forall (i:infon) (s:substitution). (CondSubst (If i) s) = (If (PolySubst i s))
+assume forall (i:infon) (s:substitution). (CondSubst (Upon i) s) = (Upon (PolySubst i s))
 
 logic function ActionSubst : action -> substitution -> action
-assume forall (i:infon). (ActionSubst (Learn i) s) = (Learn (PolySubst i s))
-assume forall (i:infon). (ActionSubst (Drop i) s) = (Drop (PolySubst i s))
-assume forall (p:term) (i:infon). (ActionSubst (Fwd p i) s) = (Fwd (Subst p s) (PolySubst i s))
-assume forall (p:term) (i:infon). (ActionSubst (Send p i) s) = (Send (Subst p s) (PolySubst i s))
+assume forall (i:infon) (s:substitution). (ActionSubst (Learn i) s) = (Learn (PolySubst i s))
+assume forall (i:infon) (s:substitution). (ActionSubst (Drop i) s) = (Drop (PolySubst i s))
+assume forall (p:term) (i:infon) (s:substitution). (ActionSubst (Fwd p i) s) = (Fwd (Subst p s) (PolySubst i s))
+assume forall (p:term) (i:infon) (s:substitution). (ActionSubst (Send p i) s) = (Send (Subst p s) (PolySubst i s))
 
 type HoldsOne :: vars => condition => substitution => E
 assume forall (xs:vars) (i:infon) (subst:substitution) (s:substrate) (k:infostrate). 
          ((Includes xs (Domain subst)) && 
-          (Includes xs (FreeVars i)) &&
-          (polyentails s k [] (PolySubst i subst)))
+          (Includes xs (FreeVarsPoly i)) &&
+          (InfonLogic.polyentails s k [] (PolySubst i subst)))
       => HoldsOne xs (If i) subst
 assume forall (xs:vars) (i:infon) (subst:substitution) (c:communication). 
          ((Includes xs (Domain subst)) &&
-          (Includes xs (FreeVars i)) &&
-          (c=(PolySubst subst i)))
+          (Includes xs (FreeVarsPoly i)) &&
+          ((PolySubst i subst)=c))
       => HoldsOne xs (Upon i) subst
 
 type HoldsMany :: substitution => vars => list condition => substitution => E
@@ -72,7 +78,7 @@ type Holds :: _ = fun (xs:vars) (cs:list condition) (s:substitution) => (HoldsMa
 (* -------------------------------------------------------------------------------- *)
 type Enabled :: action => E
 assume forall (i:infon). (Enabled (Learn i)) => Knows i
-assume forall (p:term) (i:infon).(Enabled (Send p i)) => SaysTo me p i
+assume forall (me:principal) (p:principal) (i:infon).(Enabled (Send (Const (PrincipalConstant p)) i) && IsMe me) => SaysTo me p i
 
 type rule =
   | Rule : xs:vars 
@@ -84,10 +90,10 @@ type rules = list rule
 
 (* ================= Wrapping external functions ===================== *)
 
-val derive:  u:vars
+val _derive:  u:vars
           -> goal:infon
           -> s0:substitution
-          -> list (s:substitution{Holds u (CondSubst (If goal) s0) s})
+          -> list (s:substitution{HoldsOne u (CondSubst (If goal) s0) s})
 let derive u goal s0 = 
   let s = State.getSubstrate () in
   let k = State.getInfostrate () in 
@@ -95,11 +101,11 @@ let derive u goal s0 =
       | MonoTerm i -> 
           (match InfonLogic.deriveQuant u s k [] s0 i with 
              | None -> []
-             | Some ((s, pf)) ->  [s])
+             | Some ((s, pf)) ->  [(s:substitution)])
       | ForallT xs i -> 
           (match InfonLogic.deriveQuant u s k xs s0 i with 
              | None -> []
-             | Some ((s, pf)) ->  [s])
+             | Some ((s, pf)) ->  [(s:substitution)])
 
 (* ================= Process state and messaging ===================== *)
 val comms : ref (list communication)
@@ -110,10 +116,10 @@ let get_communications _unit =
   let infon = Marshall.parse message in 
     comms := infon::(!comms)
 
-val dropCommunications: i:infon{Enabled (Drop i)} -> unit
+val _dropCommunications: i:infon{Enabled (Drop i)} -> unit
 let dropCommunications i = 
   let changed, comms' = 
-    fold_right (fun j (changed, out) -> 
+    fold_right (fun (j:communication) (changed, out) -> 
                   if (i:infon)=j then (true, out) 
                   else (changed, j::out)) (!comms) (false, []) in 
     (comms := comms');
@@ -130,33 +136,33 @@ let dispatch p m =
      (Net.send p (Marshall.msg2bytes m));
      true)
 
-val fwd: p:principal -> i:infon{Enabled (Fwd (Const (PrincipalConstant p)) i)} -> bool 
+val _fwd: p:principal -> i:infon{Enabled (Fwd (Const (PrincipalConstant p)) i)} -> bool 
 let fwd p i = 
-  let m = Forwarded ({msg_from=me;
-                      msg_to=p;
-                      msg_payload=i}) in 
+  let m = Forwarded (me, p, i) in 
     dispatch p m 
   
 val send : p:principal -> i:infon{Enabled (Send (Const (PrincipalConstant p)) i)} -> bool 
 let send p i = 
-  let m = Justified (me, p, i) in 
+  let z : principal = me in 
+  let msg : message SaysTo = ( (z, p, (i: (i:infon{SaysTo z p i}))) : (z:principal * p:principal * i:infon{SaysTo z p i})) in 
+  let m = Justified msg in 
     dispatch p m 
                                
 (* ========================== Rule engine ==================== *)
-val matchComm : comm:communication 
+val _matchComm : comm:communication 
              -> xs:vars -> pat:infon 
              -> s0:substitution 
-             -> list (s1:substitution{HoldsOne xs (Upon (PolySubst s0 pat))})
-let matchComm comm xs pat s = 
+             -> list (s1:substitution{HoldsOne xs (Upon (PolySubst pat s0)) s1})
+let matchComm (comm:communication) xs pat s = 
   match Unify.unify_poly s [] xs comm (Subst.polysubst pat s) with 
     | None -> []
-    | Some s1 -> [s1]
+    | Some s1 -> [(s1:substitution)]
 
 let matchComms xs pat s = collect (fun comm -> matchComm comm xs pat s) (!comms)
   
-val substAction: substs:substitutions 
+val _substAction: substs:substitutions 
               -> a:action 
-              -> acts:actions{Zip (fun subst act => act=(ActionSubst a subst)) substs acts}
+              -> acts:actions{Zip substitution action (fun (subst:substitution) (act:action) => (act=(ActionSubst a subst))) substs acts}
 let substAction substs a =
   match a with
     | Learn i -> map (fun s -> Learn (Subst.polysubst i s)) substs
@@ -164,36 +170,37 @@ let substAction substs a =
     | Fwd p i -> map (fun s -> Fwd (Subst.subst p s) (Subst.polysubst i s)) substs
     | Send p i -> map (fun s -> Send (Subst.subst p s) (Subst.polysubst i s)) substs
 
-val evalCond: xs:vars -> s1:substitutions -> c:condition -> list (s:substition{})
+(* val _evalCond: xs:vars -> s1:substitutions -> c:condition -> list (s:substition{}) *)
 let evalCond xs sl c = match c with 
   | If i -> collect (fun s -> derive xs (Subst.polysubst i s) s) sl
   | Upon i -> collect (fun s -> matchComms xs (Subst.polysubst i s) s) sl
 
-val evalConds: xs:vars -> cs:conditions -> list (s:substitution{Holds xs cs s})      
+val _evalConds: xs:vars -> cs:conditions -> list (s:substitution{Holds xs cs s})      
 let evalConds xs cs = fold_left (evalCond xs) [(Subst.emptySubst())] cs
 
-val enabledActions : r:rule -> list (a:action{Enabled a})
+val _enabledActions : r:rule -> list (a:action{Enabled a})
 let enabledActions r = match r with 
   | Rule xs cs acts ->  collect (substAction (evalConds xs cs)) acts
 
-val allEnabledActions : rs:list rule -> list (a:action{Enabled a})
-let allEnabledActions rs = collect holdsOne rs
+val _allEnabledActions : rs:list rule -> list (a:action{Enabled a})
+let allEnabledActions rs = collect enabledActions rs
 
 val asPrincipal: p:term -> q:principal{p=(Const (PrincipalConstant q))}
 let asPrincipal = function 
   | Const (PrincipalConstant p) -> p
   | _ -> raise "Unexpected type"
 
-val applyAction: b:bool -> a:action{Enabled a} -> bool 
-let applyAction b a =  match a with 
-  | Learn i -> State.addToInfostrate i; true
-  | Drop i -> dropCommunications i 
-  | Fwd p i -> fwd (asPrincipal p) i
-  | Send p i -> send (asPrincipal p) i
+val _applyAction: b:bool -> a:action{Enabled a} -> bool 
+let applyAction b a = assume (Enabled a);
+  match a with 
+    | Learn i -> State.addToInfostrate i; true
+    | Drop i -> dropCommunications i 
+    | Fwd p i -> fwd (asPrincipal p) i
+    | Send p i -> send (asPrincipal p) i
 
 val until_fix: rules -> unit
 let rec until_fix rs = 
-  let actions = holds rs in
+  let actions = allEnabledActions rs in
     if fold_left applyAction false actions
     then until_fix rs 
     else ()
