ModularEngine/src/LogicEngine.FStar/prog.fst
@@ -1,0 +1,24 @@
+module SampleProgram1
+open TypeHeaders
+open Types
+open Interp
+open Subst
+
+type TrustRule :: _ = 
+    (fun (xs:vars) (cs:conditions) (acts:actions) => 
+        (forall (a:action) (subst:substitution). In a acts && Holds xs cs subst => (Enabled (ActionSubst a subst))))
+
+let mkRule xs cs acts = 
+  assume (TrustRule xs cs acts);
+  Rule xs cs acts
+
+let rule1 = 
+  let vx = {name="x"; typ=Principal} in 
+  let vars = [vx] in
+  let conditions = [(If (MonoTerm (App SaidInfon [(Var vx);
+                                                  (App EmptyInfon [])])))] in 
+  let actions = [(Learn (MonoTerm (App EmptyInfon [])))] in
+    mkRule vars conditions actions
+
+
+end
